Flapjack/Test/WordToStack.lean
@@ -259,7 +259,8 @@ example :
             (2, .register 6), (3, .register 7)],
           scratch := 31, stackBase := 10 } (.longMul 0 1 2 3) =
       some (.inst (.arith (.longMul 4 5 6 7)) : StackProg Nat) := by
-  simp [wordStackArithInst, wordStackLocation, lookupNatInfo]
+  simp [wordStackArithInst, wordSpecialArithLocationsSafe,
+    wordStackLocation, lookupNatInfo]
 
 example :
     wordStackArithInst
@@ -267,7 +268,26 @@ example :
             (2, .register 6), (3, .register 7), (4, .register 8)],
           scratch := 31, stackBase := 10 } (.addCarry 0 1 2 3 4) =
       some (.inst (.arith (.addCarry 4 5 6 7 8)) : StackProg Nat) := by
-  simp [wordStackArithInst, wordStackLocation, lookupNatInfo]
+  simp [wordStackArithInst, wordSpecialArithLocationsSafe,
+    wordStackLocation, lookupNatInfo]
+
+example :
+    wordStackArithInst
+        { locations := [(0, .register 4), (1, .register 5),
+            (2, .register 4), (3, .register 7)],
+          scratch := 31, stackBase := 10 } (.longMul 0 1 2 3) =
+      (none : Option (StackProg Nat)) := by
+  simp [wordStackArithInst, wordSpecialArithLocationsSafe,
+    wordStackLocation, lookupNatInfo]
+
+example :
+    wordStackArithInst
+        { locations := [(0, .register 31), (1, .register 5),
+            (2, .register 6), (3, .register 7), (4, .register 8)],
+          scratch := 31, stackBase := 10 } (.addCarry 0 1 2 3 4) =
+      (none : Option (StackProg Nat)) := by
+  simp [wordStackArithInst, wordSpecialArithLocationsSafe,
+    wordStackLocation, lookupNatInfo]
 
 example :
     wordToStackProgNat
